09HeapMemory/HeapMemory.thy
@@ -7,56 +7,50 @@ datatype hclosure =
   | HLam "ptr list" nat
 
 datatype heap_state = 
-  HS "hclosure heap" "ptr list" "(ptr list \<times> nat) list" (code: "byte_code list")
+  HS "hclosure heap" "ptr list" "(ptr list \<times> nat) list"
 
-inductive evalh :: "heap_state \<Rightarrow> heap_state \<Rightarrow> bool" (infix "\<leadsto>\<^sub>h" 50) where
+inductive evalh :: "byte_code list \<Rightarrow> heap_state \<Rightarrow> heap_state \<Rightarrow> bool" (infix "\<tturnstile> _ \<leadsto>\<^sub>h" 50) where
   evh_lookup [simp]: "cd ! pc = BLookup x \<Longrightarrow> lookup env x = Some v \<Longrightarrow> 
-    HS h vs ((env, Suc pc) # sfs) cd \<leadsto>\<^sub>h HS h (v # vs) ((env, pc) # sfs) cd"
+    cd \<tturnstile> HS h vs ((env, Suc pc) # sfs) \<leadsto>\<^sub>h HS h (v # vs) ((env, pc) # sfs)"
 | evh_pushcon [simp]: "cd ! pc = BPushCon k \<Longrightarrow> halloc h (HConst k) = (h', v) \<Longrightarrow>
-    HS h vs ((env, Suc pc) # sfs) cd \<leadsto>\<^sub>h HS h' (v # vs) ((env, pc) # sfs) cd"
+    cd \<tturnstile> HS h vs ((env, Suc pc) # sfs) \<leadsto>\<^sub>h HS h' (v # vs) ((env, pc) # sfs)"
 | evh_pushlam [simp]: "cd ! pc = BPushLam pc' \<Longrightarrow> halloc h (HLam env pc') = (h', v) \<Longrightarrow>
-    HS h vs ((env, Suc pc) # sfs) cd \<leadsto>\<^sub>h HS h' (v # vs) ((env, pc) # sfs) cd"
+    cd \<tturnstile> HS h vs ((env, Suc pc) # sfs) \<leadsto>\<^sub>h HS h' (v # vs) ((env, pc) # sfs)"
 | evh_apply [simp]: "cd ! pc = BApply \<Longrightarrow> hlookup h v2 = HLam env' pc' \<Longrightarrow>
-    HS h (v1 # v2 # vs) ((env, Suc pc) # sfs) cd \<leadsto>\<^sub>h
-      HS h vs ((v1 # env', pc') # (env, pc) # sfs) cd"
+    cd \<tturnstile> HS h (v1 # v2 # vs) ((env, Suc pc) # sfs) \<leadsto>\<^sub>h
+      HS h vs ((v1 # env', pc') # (env, pc) # sfs)"
 | evh_return [simp]: "cd ! pc = BReturn \<Longrightarrow> 
-    HS h vs ((env, Suc pc) # sfs) cd \<leadsto>\<^sub>h HS h vs sfs cd"
+    cd \<tturnstile> HS h vs ((env, Suc pc) # sfs) \<leadsto>\<^sub>h HS h vs sfs"
 | evh_jump [simp]: "cd ! pc = BJump \<Longrightarrow> hlookup h v2 = HLam env' pc' \<Longrightarrow>
-    HS h (v1 # v2 # vs) ((env, Suc pc) # sfs) cd \<leadsto>\<^sub>h HS h vs ((v1 # env', pc') # sfs) cd"
+    cd \<tturnstile> HS h (v1 # v2 # vs) ((env, Suc pc) # sfs) \<leadsto>\<^sub>h HS h vs ((v1 # env', pc') # sfs)"
 
-theorem determinismh: "\<Sigma> \<leadsto>\<^sub>h \<Sigma>' \<Longrightarrow> \<Sigma> \<leadsto>\<^sub>h \<Sigma>'' \<Longrightarrow> \<Sigma>' = \<Sigma>''"
-proof (induction \<Sigma> \<Sigma>' rule: evalh.induct)
+theorem determinismh: "cd \<tturnstile> \<Sigma> \<leadsto>\<^sub>h \<Sigma>' \<Longrightarrow> cd \<tturnstile> \<Sigma> \<leadsto>\<^sub>h \<Sigma>'' \<Longrightarrow> \<Sigma>' = \<Sigma>''"
+proof (induction cd \<Sigma> \<Sigma>' rule: evalh.induct)
   case (evh_lookup cd pc x env v h vs sfs)
   from evh_lookup(3, 1, 2) show ?case 
-    by (induction "HS h vs ((env, Suc pc) # sfs) cd" \<Sigma>'' rule: evalh.induct) simp_all 
+    by (induction cd "HS h vs ((env, Suc pc) # sfs)" \<Sigma>'' rule: evalh.induct) simp_all 
 next
   case (evh_pushcon cd pc k h h' v vs env sfs)
   from evh_pushcon(3, 1, 2) show ?case 
-    by (induction "HS h vs ((env, Suc pc) # sfs) cd" \<Sigma>'' rule: evalh.induct) simp_all 
+    by (induction cd "HS h vs ((env, Suc pc) # sfs)" \<Sigma>'' rule: evalh.induct) simp_all 
 next
   case (evh_pushlam cd pc pc' h env h' v vs sfs)
   from evh_pushlam(3, 1, 2) show ?case 
-    by (induction "HS h vs ((env, Suc pc) # sfs) cd" \<Sigma>'' rule: evalh.induct) simp_all 
+    by (induction cd "HS h vs ((env, Suc pc) # sfs)" \<Sigma>'' rule: evalh.induct) simp_all 
 next
   case (evh_apply cd pc h v2 env' pc' v1 vs env sfs)
   from evh_apply(3, 1, 2) show ?case 
-    by (induction "HS h (v1 # v2 # vs) ((env, Suc pc) # sfs) cd" \<Sigma>'' rule: evalh.induct) 
+    by (induction cd "HS h (v1 # v2 # vs) ((env, Suc pc) # sfs)" \<Sigma>'' rule: evalh.induct) 
        simp_all 
 next
   case (evh_return cd pc h vs env sfs)
   from evh_return(2, 1) show ?case 
-    by (induction "HS h vs ((env, Suc pc) # sfs) cd" \<Sigma>'' rule: evalh.induct) simp_all 
+    by (induction cd "HS h vs ((env, Suc pc) # sfs)" \<Sigma>'' rule: evalh.induct) simp_all 
 next
   case (evh_jump cd pc h v2 env' pc' v1 vs env sfs)
   from evh_jump(3, 1, 2) show ?case 
-    by (induction "HS h (v1 # v2 # vs) ((env, Suc pc) # sfs) cd" \<Sigma>'' rule: evalh.induct) 
+    by (induction cd "HS h (v1 # v2 # vs) ((env, Suc pc) # sfs)" \<Sigma>'' rule: evalh.induct) 
        simp_all 
 qed
-
-lemma [simp]: "\<Sigma> \<leadsto>\<^sub>h \<Sigma>' \<Longrightarrow> code \<Sigma> = code \<Sigma>'"
-  by (induction \<Sigma> \<Sigma>' rule: evalh.induct) simp_all
-
-lemma [simp]: "iter (\<leadsto>\<^sub>h) \<Sigma> \<Sigma>' \<Longrightarrow> code \<Sigma> = code \<Sigma>'"
-  by (induction \<Sigma> \<Sigma>' rule: iter.induct) simp_all
 
 end
