10ChainedEnvironment/Chaining.thy
@@ -19,7 +19,7 @@ abbreviation chained_closures :: "(ptr \<times> ptr) heap \<Rightarrow> ceclosur
   "chained_closures env h \<equiv> heap_all (\<lambda>p c. chained_closure env c) h"
 
 primrec chained_state :: "chained_state \<Rightarrow> bool" where
-  "chained_state (CES h env vs sfs cd) = (
+  "chained_state (CES h env vs sfs) = (
     chain_structured env \<and> chained_closures env h \<and> chained_stack env sfs)"
 
 fun unstack_list :: "(ptr \<times> ptr) heap \<Rightarrow> ptr \<Rightarrow> ptr list" where
@@ -41,7 +41,7 @@ abbreviation unchain_stack :: "(ptr \<times> ptr) heap \<Rightarrow> (ptr \<time
   "unchain_stack env sfs \<equiv> map (unchain_frame env) sfs"
 
 primrec unchain_state :: "chained_state \<Rightarrow> heap_state" where
-  "unchain_state (CES h env vs sfs cd) = HS (unchain_heap h env) vs (unchain_stack env sfs) cd"
+  "unchain_state (CES h env vs sfs) = HS (unchain_heap h env) vs (unchain_stack env sfs)"
 
 lemma [simp]: "unchain_heap hempty env = hempty"
   by (simp add: unchain_heap_def)
@@ -87,27 +87,28 @@ lemma [simp]: "hlookup h x = CELam p pc \<Longrightarrow> hcontains h x \<Longri
     hlookup (unchain_heap h env) x = HLam (unstack_list env p) pc"
   by (simp add: unchain_heap_def)
 
-lemma unchain_state_reverse [simp]: "HS h vs sfs cd = unchain_state \<Sigma> \<Longrightarrow> 
-  \<exists>h\<^sub>c\<^sub>e env sfs\<^sub>c\<^sub>e. \<Sigma> = CES h\<^sub>c\<^sub>e env vs sfs\<^sub>c\<^sub>e cd \<and> h = unchain_heap h\<^sub>c\<^sub>e env \<and> 
+lemma unchain_state_reverse [simp]: "HS h vs sfs = unchain_state \<Sigma> \<Longrightarrow> 
+  \<exists>h\<^sub>c\<^sub>e env sfs\<^sub>c\<^sub>e. \<Sigma> = CES h\<^sub>c\<^sub>e env vs sfs\<^sub>c\<^sub>e \<and> h = unchain_heap h\<^sub>c\<^sub>e env \<and> 
     sfs = unchain_stack env sfs\<^sub>c\<^sub>e"
   by (induction \<Sigma>) simp_all
 
-theorem completece [simp]: "unchain_state \<Sigma>\<^sub>c\<^sub>e \<leadsto>\<^sub>h \<Sigma>\<^sub>h \<Longrightarrow> \<exists>\<Sigma>\<^sub>c\<^sub>e'. \<Sigma>\<^sub>c\<^sub>e \<leadsto>\<^sub>c\<^sub>e \<Sigma>\<^sub>c\<^sub>e' \<and> \<Sigma>\<^sub>h = unchain_state \<Sigma>\<^sub>c\<^sub>e'"
+theorem completece [simp]: "cd \<tturnstile> unchain_state \<Sigma>\<^sub>c\<^sub>e \<leadsto>\<^sub>h \<Sigma>\<^sub>h \<Longrightarrow> 
+    \<exists>\<Sigma>\<^sub>c\<^sub>e'. (cd \<tturnstile> \<Sigma>\<^sub>c\<^sub>e \<leadsto>\<^sub>c\<^sub>e \<Sigma>\<^sub>c\<^sub>e') \<and> \<Sigma>\<^sub>h = unchain_state \<Sigma>\<^sub>c\<^sub>e'"
   by simp
 
-lemma [simp]: "iter (\<leadsto>\<^sub>h) (unchain_state \<Sigma>\<^sub>c\<^sub>e) \<Sigma>\<^sub>h \<Longrightarrow> 
-  \<exists>\<Sigma>\<^sub>c\<^sub>e'. iter (\<leadsto>\<^sub>c\<^sub>e) \<Sigma>\<^sub>c\<^sub>e \<Sigma>\<^sub>c\<^sub>e' \<and> \<Sigma>\<^sub>h = unchain_state \<Sigma>\<^sub>c\<^sub>e'"
+lemma [simp]: "iter (\<tturnstile> cd \<leadsto>\<^sub>h) (unchain_state \<Sigma>\<^sub>c\<^sub>e) \<Sigma>\<^sub>h \<Longrightarrow> 
+  \<exists>\<Sigma>\<^sub>c\<^sub>e'. iter (\<tturnstile> cd \<leadsto>\<^sub>c\<^sub>e) \<Sigma>\<^sub>c\<^sub>e \<Sigma>\<^sub>c\<^sub>e' \<and> \<Sigma>\<^sub>h = unchain_state \<Sigma>\<^sub>c\<^sub>e'"
 proof (induction "unchain_state \<Sigma>\<^sub>c\<^sub>e" \<Sigma>\<^sub>h arbitrary: \<Sigma>\<^sub>c\<^sub>e rule: iter.induct)
   case (iter_step \<Sigma>\<^sub>h' \<Sigma>\<^sub>h'')
-  then obtain \<Sigma>\<^sub>c\<^sub>e' where "\<Sigma>\<^sub>c\<^sub>e \<leadsto>\<^sub>c\<^sub>e \<Sigma>\<^sub>c\<^sub>e' \<and> \<Sigma>\<^sub>h' = unchain_state \<Sigma>\<^sub>c\<^sub>e'" by fastforce
-  moreover with iter_step obtain \<Sigma>\<^sub>c\<^sub>e'' where "iter (\<leadsto>\<^sub>c\<^sub>e) \<Sigma>\<^sub>c\<^sub>e' \<Sigma>\<^sub>c\<^sub>e'' \<and> \<Sigma>\<^sub>h'' = unchain_state \<Sigma>\<^sub>c\<^sub>e''" 
-    by fastforce
-  ultimately have "iter (\<leadsto>\<^sub>c\<^sub>e) \<Sigma>\<^sub>c\<^sub>e \<Sigma>\<^sub>c\<^sub>e'' \<and> \<Sigma>\<^sub>h'' = unchain_state \<Sigma>\<^sub>c\<^sub>e''" by fastforce
+  then obtain \<Sigma>\<^sub>c\<^sub>e' where "(cd \<tturnstile> \<Sigma>\<^sub>c\<^sub>e \<leadsto>\<^sub>c\<^sub>e \<Sigma>\<^sub>c\<^sub>e') \<and> \<Sigma>\<^sub>h' = unchain_state \<Sigma>\<^sub>c\<^sub>e'" by fastforce
+  moreover with iter_step obtain \<Sigma>\<^sub>c\<^sub>e'' where "iter (\<tturnstile> cd \<leadsto>\<^sub>c\<^sub>e) \<Sigma>\<^sub>c\<^sub>e' \<Sigma>\<^sub>c\<^sub>e'' \<and> 
+    \<Sigma>\<^sub>h'' = unchain_state \<Sigma>\<^sub>c\<^sub>e''" by fastforce
+  ultimately have "iter (\<tturnstile> cd \<leadsto>\<^sub>c\<^sub>e) \<Sigma>\<^sub>c\<^sub>e \<Sigma>\<^sub>c\<^sub>e'' \<and> \<Sigma>\<^sub>h'' = unchain_state \<Sigma>\<^sub>c\<^sub>e''" by fastforce
   then show ?case by fastforce
 qed force+
 
-theorem correctce [simp]: "\<Sigma>\<^sub>c\<^sub>e \<leadsto>\<^sub>c\<^sub>e \<Sigma>\<^sub>c\<^sub>e' \<Longrightarrow> chained_state \<Sigma>\<^sub>c\<^sub>e \<Longrightarrow> 
-  unchain_state \<Sigma>\<^sub>c\<^sub>e \<leadsto>\<^sub>h unchain_state \<Sigma>\<^sub>c\<^sub>e'"
+theorem correctce [simp]: "cd \<tturnstile> \<Sigma>\<^sub>c\<^sub>e \<leadsto>\<^sub>c\<^sub>e \<Sigma>\<^sub>c\<^sub>e' \<Longrightarrow> chained_state \<Sigma>\<^sub>c\<^sub>e \<Longrightarrow> 
+  cd \<tturnstile> unchain_state \<Sigma>\<^sub>c\<^sub>e \<leadsto>\<^sub>h unchain_state \<Sigma>\<^sub>c\<^sub>e'"
 proof (induction \<Sigma>\<^sub>c\<^sub>e \<Sigma>\<^sub>c\<^sub>e' rule: evalce.induct)
   case (evce_apply cd pc h v2 p' pc' env v1 env' p'' vs p sfs)
   from evce_apply have "cd ! pc = BApply" by simp
@@ -116,11 +117,11 @@ proof (induction \<Sigma>\<^sub>c\<^sub>e \<Sigma>\<^sub>c\<^sub>e' rule: evalce
   from evce_apply have "chain_structured env \<and> hcontains env p \<and> chained_stack env sfs" by simp
 
   from evce_apply have "hlookup (unchain_heap h env) v2 = HLam (unstack_list env p') pc' \<Longrightarrow>
-        HS (unchain_heap h env) (v1 # v2 # vs) ((unstack_list env p, Suc pc) # unchain_stack env sfs) cd \<leadsto>\<^sub>h
-    HS (unchain_heap h env) vs ((v1 # unstack_list env p', pc') # (unstack_list env p, pc) # unchain_stack env sfs) cd" by simp
+        cd \<tturnstile> HS (unchain_heap h env) (v1 # v2 # vs) ((unstack_list env p, Suc pc) # unchain_stack env sfs) \<leadsto>\<^sub>h
+    HS (unchain_heap h env) vs ((v1 # unstack_list env p', pc') # (unstack_list env p, pc) # unchain_stack env sfs)" by simp
 
-  have "HS (unchain_heap h env) (v1 # v2 # vs) ((unstack_list env p, Suc pc) # unchain_stack env sfs) cd \<leadsto>\<^sub>h
-    HS (unchain_heap h env') vs ((unstack_list env' p'', pc') # (unstack_list env' p, pc) # unchain_stack env' sfs) cd" by simp
+  have "cd \<tturnstile> HS (unchain_heap h env) (v1 # v2 # vs) ((unstack_list env p, Suc pc) # unchain_stack env sfs) \<leadsto>\<^sub>h
+    HS (unchain_heap h env') vs ((unstack_list env' p'', pc') # (unstack_list env' p, pc) # unchain_stack env' sfs)" by simp
   then show ?case by simp
 next
   case (evce_jump cd pc h v2 p' pc' env v1 env' p'' vs p sfs)
@@ -138,17 +139,17 @@ lemma [simp]: "halloc env (v, p') = (env', p) \<Longrightarrow> chained_stack en
     chained_stack env' sfs"
   by (induction sfs) simp_all
 
-lemma [simp]: "\<Sigma>\<^sub>c\<^sub>e \<leadsto>\<^sub>c\<^sub>e \<Sigma>\<^sub>c\<^sub>e' \<Longrightarrow> chained_state \<Sigma>\<^sub>c\<^sub>e \<Longrightarrow> chained_state \<Sigma>\<^sub>c\<^sub>e'"
+lemma [simp]: "cd \<tturnstile> \<Sigma>\<^sub>c\<^sub>e \<leadsto>\<^sub>c\<^sub>e \<Sigma>\<^sub>c\<^sub>e' \<Longrightarrow> chained_state \<Sigma>\<^sub>c\<^sub>e \<Longrightarrow> chained_state \<Sigma>\<^sub>c\<^sub>e'"
   apply (induction \<Sigma>\<^sub>c\<^sub>e \<Sigma>\<^sub>c\<^sub>e' rule: evalce.induct)
   apply auto
   by simp
 
-lemma [simp]: "iter (\<leadsto>\<^sub>c\<^sub>e) \<Sigma>\<^sub>c\<^sub>e \<Sigma>\<^sub>c\<^sub>e' \<Longrightarrow> chained_state \<Sigma>\<^sub>c\<^sub>e \<Longrightarrow> 
-  iter (\<leadsto>\<^sub>h) (unchain_state \<Sigma>\<^sub>c\<^sub>e) (unchain_state \<Sigma>\<^sub>c\<^sub>e')"
+lemma [simp]: "iter (\<tturnstile> cd \<leadsto>\<^sub>c\<^sub>e) \<Sigma>\<^sub>c\<^sub>e \<Sigma>\<^sub>c\<^sub>e' \<Longrightarrow> chained_state \<Sigma>\<^sub>c\<^sub>e \<Longrightarrow> 
+  iter (\<tturnstile> cd \<leadsto>\<^sub>h) (unchain_state \<Sigma>\<^sub>c\<^sub>e) (unchain_state \<Sigma>\<^sub>c\<^sub>e')"
 proof (induction \<Sigma>\<^sub>c\<^sub>e \<Sigma>\<^sub>c\<^sub>e' rule: iter.induct)
   case (iter_step \<Sigma>\<^sub>c\<^sub>e \<Sigma>\<^sub>c\<^sub>e' \<Sigma>\<^sub>c\<^sub>e'')
-  hence "iter (\<leadsto>\<^sub>h) (unchain_state \<Sigma>\<^sub>c\<^sub>e') (unchain_state \<Sigma>\<^sub>c\<^sub>e'')" by simp
-  moreover from iter_step have "unchain_state \<Sigma>\<^sub>c\<^sub>e \<leadsto>\<^sub>h unchain_state \<Sigma>\<^sub>c\<^sub>e'" by simp
+  hence "iter (\<tturnstile> cd \<leadsto>\<^sub>h) (unchain_state \<Sigma>\<^sub>c\<^sub>e') (unchain_state \<Sigma>\<^sub>c\<^sub>e'')" by simp
+  moreover from iter_step have "cd \<tturnstile> unchain_state \<Sigma>\<^sub>c\<^sub>e \<leadsto>\<^sub>h unchain_state \<Sigma>\<^sub>c\<^sub>e'" by simp
   ultimately show ?case by simp
 qed simp_all
 
