11FlatMemory/FlatMemory.thy
@@ -3,7 +3,7 @@ theory FlatMemory
 begin
 
 datatype flat_state = 
-  FS "nat heap" "ptr heap" "ptr list" "nat list" (code: "byte_code list")
+  FS "nat heap" "ptr heap" "ptr list" "nat list"
 
 fun get_closure :: "nat heap \<Rightarrow> nat \<Rightarrow> ceclosure" where
   "get_closure h p = (case hlookup h p of
@@ -16,53 +16,47 @@ fun flat_lookup :: "ptr heap \<Rightarrow> ptr \<Rightarrow> nat \<rightharpoonu
 | "flat_lookup h (Suc (Suc p)) 0 = Some (hlookup h p)"
 | "flat_lookup h (Suc (Suc p)) (Suc x) = flat_lookup h (hlookup h (Suc p)) x"
 
-inductive evalf :: "flat_state \<Rightarrow> flat_state \<Rightarrow> bool" (infix "\<leadsto>\<^sub>f" 50) where
+inductive evalf :: "byte_code list \<Rightarrow> flat_state \<Rightarrow> flat_state \<Rightarrow> bool" (infix "\<tturnstile> _ \<leadsto>\<^sub>f" 50) where
   evf_lookup [simp]: "cd ! pc = BLookup x \<Longrightarrow> flat_lookup env p x = Some v \<Longrightarrow> 
-    FS h env vs (Suc pc # p # sfs) cd \<leadsto>\<^sub>f FS h env (v # vs) (pc # p # sfs) cd"
+    cd \<tturnstile> FS h env vs (Suc pc # p # sfs) \<leadsto>\<^sub>f FS h env (v # vs) (pc # p # sfs)"
 | evf_pushcon [simp]: "cd ! pc = BPushCon k \<Longrightarrow> halloc_list h [0, k, 0] = (h', v) \<Longrightarrow>
-    FS h env vs (Suc pc # p # sfs) cd \<leadsto>\<^sub>f FS h' env (v # vs) (pc # p # sfs) cd"
+    cd \<tturnstile> FS h env vs (Suc pc # p # sfs) \<leadsto>\<^sub>f FS h' env (v # vs) (pc # p # sfs)"
 | evf_pushlam [simp]: "cd ! pc = BPushLam pc' \<Longrightarrow> halloc_list h [1, p, pc'] = (h', v) \<Longrightarrow> 
-    FS h env vs (Suc pc # p # sfs) cd \<leadsto>\<^sub>f FS h' env (v # vs) (pc # p # sfs) cd"
+    cd \<tturnstile> FS h env vs (Suc pc # p # sfs) \<leadsto>\<^sub>f FS h' env (v # vs) (pc # p # sfs)"
 | evf_apply [simp]: "cd ! pc = BApply \<Longrightarrow> get_closure h v2 = CELam p' pc' \<Longrightarrow>
     halloc env v1 = (env1, p1) \<Longrightarrow> halloc env1 p' = (env2, p2) \<Longrightarrow> 
-      FS h env (v1 # v2 # vs) (Suc pc # p # sfs) cd \<leadsto>\<^sub>f 
-        FS h env2 vs (pc' # Suc p2 # pc # p # sfs) cd"
-| evf_return [simp]: "cd ! pc = BReturn \<Longrightarrow> FS h env vs (Suc pc # p # sfs) cd \<leadsto>\<^sub>f FS h env vs sfs cd"
+      cd \<tturnstile> FS h env (v1 # v2 # vs) (Suc pc # p # sfs) \<leadsto>\<^sub>f 
+        FS h env2 vs (pc' # Suc p2 # pc # p # sfs)"
+| evf_return [simp]: "cd ! pc = BReturn \<Longrightarrow> cd \<tturnstile> FS h env vs (Suc pc # p # sfs) \<leadsto>\<^sub>f FS h env vs sfs"
 | evf_jump [simp]: "cd ! pc = BJump \<Longrightarrow> get_closure h v2 = CELam p' pc' \<Longrightarrow>
     halloc env v1 = (env1, p1) \<Longrightarrow> halloc env1 p' = (env2, p2) \<Longrightarrow> 
-      FS h env (v1 # v2 # vs) (Suc pc # p # sfs) cd \<leadsto>\<^sub>f FS h env2 vs (pc' # Suc p2 # sfs) cd"
+      cd \<tturnstile> FS h env (v1 # v2 # vs) (Suc pc # p # sfs) \<leadsto>\<^sub>f FS h env2 vs (pc' # Suc p2 # sfs)"
 
-theorem determinismf: "\<Sigma> \<leadsto>\<^sub>f \<Sigma>' \<Longrightarrow> \<Sigma> \<leadsto>\<^sub>f \<Sigma>'' \<Longrightarrow> \<Sigma>' = \<Sigma>''"
+theorem determinismf: "cd \<tturnstile> \<Sigma> \<leadsto>\<^sub>f \<Sigma>' \<Longrightarrow> cd \<tturnstile> \<Sigma> \<leadsto>\<^sub>f \<Sigma>'' \<Longrightarrow> \<Sigma>' = \<Sigma>''"
 proof (induction \<Sigma> \<Sigma>' rule: evalf.induct)
   case (evf_lookup cd pc x env p v h vs sfs)
   from evf_lookup(3, 1, 2) show ?case 
-    by (induction "FS h env vs (Suc pc # p # sfs) cd" \<Sigma>'' rule: evalf.induct) simp_all 
+    by (induction cd "FS h env vs (Suc pc # p # sfs)" \<Sigma>'' rule: evalf.induct) simp_all 
 next
   case (evf_pushcon cd pc k h h' v env vs p sfs)
   from evf_pushcon(3, 1, 2) show ?case 
-    by (induction "FS h env vs (Suc pc # p # sfs) cd" \<Sigma>'' rule: evalf.induct) simp_all 
+    by (induction cd "FS h env vs (Suc pc # p # sfs)" \<Sigma>'' rule: evalf.induct) simp_all 
 next
   case (evf_pushlam cd pc pc' h p h' v env vs sfs)
   from evf_pushlam(3, 1, 2) show ?case 
-    by (induction "FS h env vs (Suc pc # p # sfs) cd" \<Sigma>'' rule: evalf.induct) simp_all 
+    by (induction cd "FS h env vs (Suc pc # p # sfs)" \<Sigma>'' rule: evalf.induct) simp_all 
 next
   case (evf_apply cd pc h v2 p' pc' env v1 env1 p1 env2 p2 vs p sfs)
   from evf_apply(5, 1, 2, 3, 4) show ?case 
-    by (induction "FS h env (v1 # v2 # vs) (Suc pc # p # sfs) cd" \<Sigma>'' rule: evalf.induct) simp_all 
+    by (induction cd "FS h env (v1 # v2 # vs) (Suc pc # p # sfs)" \<Sigma>'' rule: evalf.induct) simp_all 
 next
   case (evf_return cd pc h env vs p sfs)
   from evf_return(2, 1) show ?case 
-    by (induction "FS h env vs (Suc pc # p # sfs) cd" \<Sigma>'' rule: evalf.induct) simp_all 
+    by (induction cd "FS h env vs (Suc pc # p # sfs)" \<Sigma>'' rule: evalf.induct) simp_all 
 next
   case (evf_jump cd pc h v2 p' pc' env v1 env1 p1 env2 p2 vs p sfs)
   from evf_jump(5, 1, 2, 3, 4) show ?case 
-    by (induction "FS h env (v1 # v2 # vs) (Suc pc # p # sfs) cd" \<Sigma>'' rule: evalf.induct) simp_all 
+    by (induction cd "FS h env (v1 # v2 # vs) (Suc pc # p # sfs)" \<Sigma>'' rule: evalf.induct) simp_all 
 qed
-
-lemma [simp]: "\<Sigma> \<leadsto>\<^sub>f \<Sigma>' \<Longrightarrow> code \<Sigma> = code \<Sigma>'"
-  by (induction \<Sigma> \<Sigma>' rule: evalf.induct) simp_all
-
-lemma [simp]: "iter (\<leadsto>\<^sub>f) \<Sigma> \<Sigma>' \<Longrightarrow> code \<Sigma> = code \<Sigma>'"
-  by (induction \<Sigma> \<Sigma>' rule: iter.induct) simp_all
 
 end
