11FlatMemory/MemoryFlattening.thy
@@ -22,8 +22,8 @@ abbreviation flatten_stack :: "(ptr \<times> nat) list \<Rightarrow> nat list" w
   "flatten_stack sfs \<equiv> concat (map flatten_frame sfs)"
 
 primrec flatten :: "chained_state \<Rightarrow> flat_state" where
-  "flatten (CES h env vs sfs cd) = 
-      FS (flatten_values h) (flatten_environment env) vs (flatten_stack sfs) cd"
+  "flatten (CES h env vs sfs) = 
+      FS (flatten_values h) (flatten_environment env) vs (flatten_stack sfs)"
 
 lemma [simp]: "get_closure (flatten_values h) v = hlookup h v"
   by simp
@@ -44,10 +44,10 @@ lemma flatten_halloc [simp]: "halloc h c = (h', v) \<Longrightarrow>
     halloc_list (flatten_values h) (flatten_closure c) = (flatten_values h', v)"
   by simp
 
-theorem correctf: "flatten \<Sigma>\<^sub>c\<^sub>e \<leadsto>\<^sub>f \<Sigma>\<^sub>f' \<Longrightarrow> \<exists>\<Sigma>\<^sub>c\<^sub>e'. \<Sigma>\<^sub>c\<^sub>e \<leadsto>\<^sub>c\<^sub>e \<Sigma>\<^sub>c\<^sub>e' \<and> flatten \<Sigma>\<^sub>c\<^sub>e' = \<Sigma>\<^sub>f'" 
+theorem correctf: "cd \<tturnstile> flatten \<Sigma>\<^sub>c\<^sub>e \<leadsto>\<^sub>f \<Sigma>\<^sub>f' \<Longrightarrow> \<exists>\<Sigma>\<^sub>c\<^sub>e'. (cd \<tturnstile> \<Sigma>\<^sub>c\<^sub>e \<leadsto>\<^sub>c\<^sub>e \<Sigma>\<^sub>c\<^sub>e') \<and> flatten \<Sigma>\<^sub>c\<^sub>e' = \<Sigma>\<^sub>f'" 
   by simp
 
-theorem completef [simp]: "\<Sigma>\<^sub>c\<^sub>e \<leadsto>\<^sub>c\<^sub>e \<Sigma>\<^sub>c\<^sub>e' \<Longrightarrow> flatten \<Sigma>\<^sub>c\<^sub>e \<leadsto>\<^sub>f flatten \<Sigma>\<^sub>c\<^sub>e'" 
+theorem completef [simp]: "cd \<tturnstile> \<Sigma>\<^sub>c\<^sub>e \<leadsto>\<^sub>c\<^sub>e \<Sigma>\<^sub>c\<^sub>e' \<Longrightarrow> cd \<tturnstile> flatten \<Sigma>\<^sub>c\<^sub>e \<leadsto>\<^sub>f flatten \<Sigma>\<^sub>c\<^sub>e'" 
 proof (induction \<Sigma>\<^sub>c\<^sub>e \<Sigma>\<^sub>c\<^sub>e' rule: evalce.induct)
   case (evce_pushcon cd pc k h h' v env vs p sfs)
   moreover hence "halloc_list (flatten_values h) [0, k, 0] = (flatten_values h', v)" 
@@ -66,11 +66,12 @@ next
   then show ?case by simp
 qed simp_all
 
-lemma completef_iter [simp]: "iter (\<leadsto>\<^sub>c\<^sub>e) \<Sigma>\<^sub>c\<^sub>e \<Sigma>\<^sub>c\<^sub>e' \<Longrightarrow> iter (\<leadsto>\<^sub>f) (flatten \<Sigma>\<^sub>c\<^sub>e) (flatten \<Sigma>\<^sub>c\<^sub>e')"
+lemma completef_iter [simp]: "iter (\<tturnstile> cd \<leadsto>\<^sub>c\<^sub>e) \<Sigma>\<^sub>c\<^sub>e \<Sigma>\<^sub>c\<^sub>e' \<Longrightarrow> 
+  iter (\<tturnstile> cd \<leadsto>\<^sub>f) (flatten \<Sigma>\<^sub>c\<^sub>e) (flatten \<Sigma>\<^sub>c\<^sub>e')"
 proof (induction \<Sigma>\<^sub>c\<^sub>e \<Sigma>\<^sub>c\<^sub>e' rule: iter.induct)
   case (iter_step \<Sigma>\<^sub>c\<^sub>e \<Sigma>\<^sub>c\<^sub>e' \<Sigma>\<^sub>c\<^sub>e'')
-  hence "iter (\<leadsto>\<^sub>f) (flatten \<Sigma>\<^sub>c\<^sub>e') (flatten \<Sigma>\<^sub>c\<^sub>e'')" by simp
-  moreover from iter_step have "flatten \<Sigma>\<^sub>c\<^sub>e \<leadsto>\<^sub>f flatten \<Sigma>\<^sub>c\<^sub>e'" by simp
+  hence "iter (\<tturnstile> cd \<leadsto>\<^sub>f) (flatten \<Sigma>\<^sub>c\<^sub>e') (flatten \<Sigma>\<^sub>c\<^sub>e'')" by simp
+  moreover from iter_step have "cd \<tturnstile> flatten \<Sigma>\<^sub>c\<^sub>e \<leadsto>\<^sub>f flatten \<Sigma>\<^sub>c\<^sub>e'" by simp
   ultimately show ?case by simp
 qed simp_all
 
