12UnstructuredMemory/Unstructuring.thy
@@ -3,12 +3,12 @@ theory Unstructuring
 begin
 
 fun restructure :: "unstr_state \<Rightarrow> flat_state" where
-  "restructure (US h hp x p e ep vs vp sh sp 0 cd) = 
-    FS (H h hp) (H e ep) (listify' vs vp) [] cd"
-| "restructure (US h hp x p e ep vs vp sh sp (Suc pc) cd) = 
-    FS (H h hp) (H e ep) (listify' vs vp) (Suc pc # listify' sh sp) cd"
+  "restructure (US h hp x p e ep vs vp sh sp 0) = 
+    FS (H h hp) (H e ep) (listify' vs vp) []"
+| "restructure (US h hp x p e ep vs vp sh sp (Suc pc)) = 
+    FS (H h hp) (H e ep) (listify' vs vp) (Suc pc # listify' sh sp)"
 
-theorem completeu [simp]: "\<Sigma>\<^sub>u \<leadsto>\<^sub>u \<Sigma>\<^sub>u' \<Longrightarrow> iter (\<leadsto>\<^sub>f) (restructure \<Sigma>\<^sub>u) (restructure \<Sigma>\<^sub>u')"
+theorem completeu [simp]: "cd \<tturnstile> \<Sigma>\<^sub>u \<leadsto>\<^sub>u \<Sigma>\<^sub>u' \<Longrightarrow> iter (\<tturnstile> cd \<leadsto>\<^sub>f) (restructure \<Sigma>\<^sub>u) (restructure \<Sigma>\<^sub>u')"
 proof (induction \<Sigma>\<^sub>u \<Sigma>\<^sub>u' rule: evalu.induct)
   case (evu_lookup_zero cd pc x h hp p e ep vs vp sh sp)
   then show ?case by simp
@@ -29,18 +29,18 @@ next
   then show ?case by simp
 qed simp_all
 
-lemma [dest]: "FS h env vs sfs cd = restructure \<Sigma> \<Longrightarrow> \<exists>h' hp x p e ep vs' vp sh sp pc. 
-  \<Sigma> = US h' hp x p e ep vs' vp sh sp pc cd \<and> h = H h' hp \<and> env = H e ep \<and> vs = listify' vs' vp \<and> 
+lemma [dest]: "FS h env vs sfs = restructure \<Sigma> \<Longrightarrow> \<exists>h' hp x p e ep vs' vp sh sp pc. 
+  \<Sigma> = US h' hp x p e ep vs' vp sh sp pc \<and> h = H h' hp \<and> env = H e ep \<and> vs = listify' vs' vp \<and> 
     ((pc = 0 \<and> sfs = []) \<or> (\<exists>pc'. pc = Suc pc' \<and> sfs = pc # listify' sh sp))"
   by (induction \<Sigma> rule: restructure.induct) simp_all
 
-theorem correctu [simp]: "restructure \<Sigma>\<^sub>u \<leadsto>\<^sub>f \<Sigma>\<^sub>f' \<Longrightarrow> 
-    \<exists>\<Sigma>\<^sub>u'. iter (\<leadsto>\<^sub>u) \<Sigma>\<^sub>u \<Sigma>\<^sub>u' \<and> \<Sigma>\<^sub>f' = restructure \<Sigma>\<^sub>u'"
+theorem correctu [simp]: "cd \<tturnstile> restructure \<Sigma>\<^sub>u \<leadsto>\<^sub>f \<Sigma>\<^sub>f' \<Longrightarrow> 
+    \<exists>\<Sigma>\<^sub>u'. iter (\<tturnstile> cd \<leadsto>\<^sub>u) \<Sigma>\<^sub>u \<Sigma>\<^sub>u' \<and> \<Sigma>\<^sub>f' = restructure \<Sigma>\<^sub>u'"
 proof (induction "restructure \<Sigma>\<^sub>u" \<Sigma>\<^sub>f' rule: evalf.induct)
   case (evf_lookup cd pc x env p v h vs sfs)
-  hence "FS h env vs (Suc pc # p # sfs) cd = restructure \<Sigma>\<^sub>u" by simp
+  hence "FS h env vs (Suc pc # p # sfs) = restructure \<Sigma>\<^sub>u" by simp
   then obtain h' hp xx pp e ep vs' vp sh sp where S: "
-    \<Sigma>\<^sub>u = US h' hp xx pp e ep vs' vp sh sp (Suc pc) cd \<and> h = H h' hp \<and> env = H e ep \<and> 
+    \<Sigma>\<^sub>u = US h' hp xx pp e ep vs' vp sh sp (Suc pc) \<and> h = H h' hp \<and> env = H e ep \<and> 
       vs = listify' vs' vp \<and> p # sfs = listify' sh sp" by fastforce
 
 
@@ -49,7 +49,7 @@ proof (induction "restructure \<Sigma>\<^sub>u" \<Sigma>\<^sub>f' rule: evalf.in
 
 
 
-  have "iter (\<leadsto>\<^sub>u) (US h' hp xx pp e ep vs' vp sh sp (Suc pc) cd) \<Sigma>\<^sub>u' \<and> FS h env (v # vs) (pc # p # sfs) cd = restructure \<Sigma>\<^sub>u'" by simp
+  have "iter (\<tturnstile> cd \<leadsto>\<^sub>u) (US h' hp xx pp e ep vs' vp sh sp (Suc pc)) \<Sigma>\<^sub>u' \<and> FS h env (v # vs) (pc # p # sfs) = restructure \<Sigma>\<^sub>u'" by simp
   with S show ?case by blast
 next
   case (evf_pushcon cd pc k h h' v env vs p sfs)
@@ -68,8 +68,8 @@ next
   then show ?case by simp
 qed
 
-theorem correctu_iter [simp]: "iter (\<leadsto>\<^sub>f) (restructure \<Sigma>\<^sub>u) \<Sigma>\<^sub>f' \<Longrightarrow> 
-    \<exists>\<Sigma>\<^sub>u'. iter (\<leadsto>\<^sub>u) \<Sigma>\<^sub>u \<Sigma>\<^sub>u' \<and> \<Sigma>\<^sub>f' = restructure \<Sigma>\<^sub>u'"
+theorem correctu_iter [simp]: "iter (\<tturnstile> cd \<leadsto>\<^sub>f) (restructure \<Sigma>\<^sub>u) \<Sigma>\<^sub>f' \<Longrightarrow> 
+    \<exists>\<Sigma>\<^sub>u'. iter (\<tturnstile> cd \<leadsto>\<^sub>u) \<Sigma>\<^sub>u \<Sigma>\<^sub>u' \<and> \<Sigma>\<^sub>f' = restructure \<Sigma>\<^sub>u'"
   by (induction "restructure \<Sigma>\<^sub>u" \<Sigma>\<^sub>f' arbitrary: \<Sigma>\<^sub>u rule: iter.induct)
      (force, metis correctu iter_append)
 
