Compiler.thy
@@ -17,8 +17,8 @@ qed
 
 theorem tc_terminationn: "compile e = Some cd \<Longrightarrow> 
   \<exists>v. valn v \<and> e \<Down> v \<and> 
-    (\<exists>h hp e ep v\<^sub>u s. iter (\<leadsto>\<^sub>u) (US nmem 0 0 0 nmem 0 nmem 0 (nmem(0 := 0)) 1 (length cd) cd) 
-      (US h hp 0 0 e ep v\<^sub>u 1 s 0 0 cd) \<and> print_uclosure h (v\<^sub>u 0) = print_nexpr v)"
+    (\<exists>h hp e ep v\<^sub>u s. iter (\<tturnstile> cd \<leadsto>\<^sub>u) (US nmem 0 0 0 nmem 0 nmem 0 (nmem(0 := 0)) 1 (length cd)) 
+      (US h hp 0 0 e ep v\<^sub>u 1 s 0 0) \<and> print_uclosure h (v\<^sub>u 0) = print_nexpr v)"
 proof -
   assume C: "compile e = Some cd"
   then obtain e\<^sub>t t where T: "typecheck e = Some (e\<^sub>t, t)" by fastforce
@@ -47,51 +47,50 @@ proof -
   hence ET: "iter (\<leadsto>\<^sub>t\<^sub>c\<^sub>o) (TCOS [] [([], tco_cd (encode (convert e\<^sub>t)), tco_r (encode (convert e\<^sub>t)))]) 
     (TCOS [tco_val (encode_closure c)] [])" by simp
   from C T have "(flatten_code \<circ> tco \<circ> encode \<circ> convert) e\<^sub>t = cd" by simp
-  hence UB: "unflatten_state (BS [] [([], length cd)] cd) = 
+  hence UB: "unflatten_state cd (BS [] [([], length cd)]) = 
     TCOS [] [([], tco_cd (encode (convert e\<^sub>t)), tco_r (encode (convert e\<^sub>t)))]" 
       by (auto simp add: tco_def simp del: flatten_code.simps)
-  from C have "orderly_state (BS [] [([], length cd)] cd)" by auto
-  with ET UB obtain v\<^sub>b where EB: 
-    "iter (\<leadsto>\<^sub>b) (BS [] [([], length cd)] cd) (BS [v\<^sub>b] [] cd) \<and> 
-      tco_val (encode_closure c) = unflatten_closure cd v\<^sub>b" 
-    by (metis evalb_end byte_code_state.sel(3))
+  from C have "orderly_state cd (BS [] [([], length cd)])" by auto
+  with ET UB obtain v\<^sub>b where EB: "iter (\<tturnstile> cd \<leadsto>\<^sub>b) (BS [] [([], length cd)]) (BS [v\<^sub>b] []) \<and> 
+    tco_val (encode_closure c) = unflatten_closure cd v\<^sub>b" by (metis evalb_end)
   hence "print_bclosure v\<^sub>b = print_tco_closure (tco_val (encode_closure c))" by simp
   with VC have VB: "print_bclosure v\<^sub>b = print_nexpr (erase v\<^sub>t)" by simp
-  from EB obtain \<Sigma>\<^sub>h' where EH: "iter (\<leadsto>\<^sub>h) (HS hempty [] [([], length cd)] cd) \<Sigma>\<^sub>h' \<and> 
-    BS [v\<^sub>b] [] cd = unheap \<Sigma>\<^sub>h'" by fastforce
-  then obtain h\<^sub>h v\<^sub>h where SH: "\<Sigma>\<^sub>h' = HS h\<^sub>h [v\<^sub>h] [] cd \<and> v\<^sub>b = unheap_closure h\<^sub>h v\<^sub>h" 
+  from EB obtain \<Sigma>\<^sub>h' where EH: "iter (\<tturnstile> cd \<leadsto>\<^sub>h) (HS hempty [] [([], length cd)]) \<Sigma>\<^sub>h' \<and> 
+    BS [v\<^sub>b] [] = unheap \<Sigma>\<^sub>h'" by fastforce
+  then obtain h\<^sub>h v\<^sub>h where SH: "\<Sigma>\<^sub>h' = HS h\<^sub>h [v\<^sub>h] [] \<and> v\<^sub>b = unheap_closure h\<^sub>h v\<^sub>h" 
     using unheap_empty by blast
   with VB have VH: "print_hclosure (hlookup h\<^sub>h v\<^sub>h) = print_nexpr (erase v\<^sub>t)" by simp
-  have HS: "heap_structured (HS hempty [] [([], length cd)] cd)" by simp
-  have CES: "unchain_state (CES hempty hempty [] [(0, length cd)] cd) = 
-    HS hempty [] [([], length cd)] cd" by simp
-  with EH SH obtain \<Sigma>\<^sub>c\<^sub>e' where ECE: "iter (\<leadsto>\<^sub>c\<^sub>e) (CES hempty hempty [] [(0, length cd)] cd) \<Sigma>\<^sub>c\<^sub>e' \<and> 
-    HS h\<^sub>h [v\<^sub>h] [] cd = unchain_state \<Sigma>\<^sub>c\<^sub>e'" by fastforce
-  then obtain h\<^sub>c\<^sub>e env\<^sub>h where VCE: "\<Sigma>\<^sub>c\<^sub>e' = CES h\<^sub>c\<^sub>e env\<^sub>h [v\<^sub>h] [] cd \<and> h\<^sub>h = unchain_heap h\<^sub>c\<^sub>e env\<^sub>h" 
+  have HS: "heap_structured (HS hempty [] [([], length cd)])" by simp
+  have CES: "unchain_state (CES hempty hempty [] [(0, length cd)]) = 
+    HS hempty [] [([], length cd)]" by simp
+  with EH SH obtain \<Sigma>\<^sub>c\<^sub>e' where ECE: "iter (\<tturnstile> cd \<leadsto>\<^sub>c\<^sub>e) (CES hempty hempty [] [(0, length cd)]) \<Sigma>\<^sub>c\<^sub>e' \<and> 
+    HS h\<^sub>h [v\<^sub>h] [] = unchain_state \<Sigma>\<^sub>c\<^sub>e'" by fastforce
+  then obtain h\<^sub>c\<^sub>e env\<^sub>h where VCE: "\<Sigma>\<^sub>c\<^sub>e' = CES h\<^sub>c\<^sub>e env\<^sub>h [v\<^sub>h] [] \<and> h\<^sub>h = unchain_heap h\<^sub>c\<^sub>e env\<^sub>h" 
     by (metis unchain_state_reverse map_is_Nil_conv)
   with VH have PCE: "print_ceclosure (hlookup h\<^sub>c\<^sub>e v\<^sub>h) = print_nexpr (erase v\<^sub>t)" by (metis print_ce)
-  from ECE VCE have "iter (\<leadsto>\<^sub>f) (flatten (CES hempty hempty [] [(0, length cd)] cd))
-    (flatten (CES h\<^sub>c\<^sub>e env\<^sub>h [v\<^sub>h] [] cd))" by (metis completef_iter)
-  hence EF: "iter (\<leadsto>\<^sub>f) (FS (H nmem 0) (H nmem 0) [] [length cd, 0] cd)
-     (FS (flatten_values h\<^sub>c\<^sub>e) (flatten_environment env\<^sub>h) [v\<^sub>h] [] cd)" by (simp add: hempty_def)
+  from ECE VCE have "iter (\<tturnstile> cd \<leadsto>\<^sub>f) (flatten (CES hempty hempty [] [(0, length cd)]))
+    (flatten (CES h\<^sub>c\<^sub>e env\<^sub>h [v\<^sub>h] []))" by (metis completef_iter)
+  hence EF: "iter (\<tturnstile> cd \<leadsto>\<^sub>f) (FS (H nmem 0) (H nmem 0) [] [length cd, 0])
+     (FS (flatten_values h\<^sub>c\<^sub>e) (flatten_environment env\<^sub>h) [v\<^sub>h] [])" by (simp add: hempty_def)
   from PCE have PF: "print_ceclosure (get_closure (flatten_values h\<^sub>c\<^sub>e) v\<^sub>h) = print_nexpr (erase v\<^sub>t)" 
     by (simp del: get_closure.simps)
   from C have "cd \<noteq> []" by auto
-  with EF have "\<exists>\<Sigma>\<^sub>u'. iter (\<leadsto>\<^sub>u) (US nmem 0 0 0 nmem 0 nmem 0 (nmem(0 := 0)) 1 (length cd) cd) \<Sigma>\<^sub>u' \<and> 
-    FS (flatten_values h\<^sub>c\<^sub>e) (flatten_environment env\<^sub>h) [v\<^sub>h] [] cd = restructure \<Sigma>\<^sub>u'" 
-      by (cases cd) simp_all
+  with EF have "\<exists>\<Sigma>\<^sub>u'. 
+    iter (\<tturnstile> cd \<leadsto>\<^sub>u) (US nmem 0 0 0 nmem 0 nmem 0 (nmem(0 := 0)) 1 (length cd)) \<Sigma>\<^sub>u' \<and> 
+      FS (flatten_values h\<^sub>c\<^sub>e) (flatten_environment env\<^sub>h) [v\<^sub>h] [] = restructure \<Sigma>\<^sub>u'"
+        by (cases cd) simp_all
   then obtain \<Sigma>\<^sub>u' where 
-    "iter (\<leadsto>\<^sub>u) (US nmem 0 0 0 nmem 0 nmem 0 (nmem(0 := 0)) 1 (length cd) cd) \<Sigma>\<^sub>u' \<and> 
-      FS (flatten_values h\<^sub>c\<^sub>e) (flatten_environment env\<^sub>h) [v\<^sub>h] [] cd = restructure \<Sigma>\<^sub>u'" by blast
+    "iter (\<tturnstile> cd \<leadsto>\<^sub>u) (US nmem 0 0 0 nmem 0 nmem 0 (nmem(0 := 0)) 1 (length cd)) \<Sigma>\<^sub>u' \<and> 
+      FS (flatten_values h\<^sub>c\<^sub>e) (flatten_environment env\<^sub>h) [v\<^sub>h] [] = restructure \<Sigma>\<^sub>u'" by blast
   moreover then obtain h\<^sub>u hp\<^sub>u x\<^sub>u p\<^sub>u e\<^sub>u ep\<^sub>u vs\<^sub>u vp\<^sub>u sh\<^sub>u sp\<^sub>u where VU:
-    "\<Sigma>\<^sub>u' = US h\<^sub>u hp\<^sub>u x\<^sub>u p\<^sub>u e\<^sub>u ep\<^sub>u vs\<^sub>u vp\<^sub>u sh\<^sub>u sp\<^sub>u 0 cd \<and> flatten_values h\<^sub>c\<^sub>e = H h\<^sub>u hp\<^sub>u \<and> 
+    "\<Sigma>\<^sub>u' = US h\<^sub>u hp\<^sub>u x\<^sub>u p\<^sub>u e\<^sub>u ep\<^sub>u vs\<^sub>u vp\<^sub>u sh\<^sub>u sp\<^sub>u 0 \<and> flatten_values h\<^sub>c\<^sub>e = H h\<^sub>u hp\<^sub>u \<and> 
       flatten_environment env\<^sub>h = H e\<^sub>u ep\<^sub>u \<and> listify' vs\<^sub>u vp\<^sub>u = v\<^sub>h # []" by auto
   moreover hence VSU: "vs\<^sub>u 0 = v\<^sub>h \<and> vp\<^sub>u = 1" by auto
-  ultimately have "iter (\<leadsto>\<^sub>u) (US nmem 0 0 0 nmem 0 nmem 0 (nmem(0 := 0)) 1 (length cd) cd) 
-    (US h\<^sub>u hp\<^sub>u x\<^sub>u p\<^sub>u e\<^sub>u ep\<^sub>u vs\<^sub>u 1 sh\<^sub>u sp\<^sub>u 0 cd)" by simp
+  ultimately have "iter (\<tturnstile> cd \<leadsto>\<^sub>u) (US nmem 0 0 0 nmem 0 nmem 0 (nmem(0 := 0)) 1 (length cd)) 
+    (US h\<^sub>u hp\<^sub>u x\<^sub>u p\<^sub>u e\<^sub>u ep\<^sub>u vs\<^sub>u 1 sh\<^sub>u sp\<^sub>u 0)" by simp
   moreover hence "x\<^sub>u = 0 \<and> p\<^sub>u = 0 \<and> sp\<^sub>u = 0" by (metis evalu_clears_regs)
-  ultimately have EU: "iter (\<leadsto>\<^sub>u) (US nmem 0 0 0 nmem 0 nmem 0 (nmem(0 := 0)) 1 (length cd) cd) 
-    (US h\<^sub>u hp\<^sub>u 0 0 e\<^sub>u ep\<^sub>u vs\<^sub>u 1 sh\<^sub>u 0 0 cd)" by simp
+  ultimately have EU: "iter (\<tturnstile> cd \<leadsto>\<^sub>u) (US nmem 0 0 0 nmem 0 nmem 0 (nmem(0 := 0)) 1 (length cd)) 
+    (US h\<^sub>u hp\<^sub>u 0 0 e\<^sub>u ep\<^sub>u vs\<^sub>u 1 sh\<^sub>u 0 0)" by simp
 
 
 
